TypingContexts.v
@@ -59,9 +59,62 @@ Theorem restriction_makes_subset :
     VarSet.Subset (g -- v) g.
 Proof. Admitted.
 
+Theorem restriction_makes_variable_notin :
+  forall g : ty_ctx,
+  forall v : var,
+    ~(VarSet.In v (g -- v)).
+Proof. Admitted.
+
+Theorem restr_of_notin_makes_equal :
+  forall g : ty_ctx,
+  forall x : var,
+  forall x_gfree : ~(VarSet.In x (bound_variables g)),
+    g = (g -- x).
+Proof. Admitted.
+
+Theorem disj_vars_assoc :
+  forall g1 g2 g3 : ty_ctx,
+  forall disj_g12 : disj_vars g1 g2,
+  forall eq_g23 : g2 = g3,
+    disj_vars g1 g3.
+Proof. Admitted.
+
+Theorem ctx_union_of_eql :
+  forall g1 g2 g3 : ty_ctx,
+  forall disj_g12 : disj_vars g1 g2,
+  forall disj_g13 : disj_vars g1 g3,
+  forall eq_23 : g2 = g3,
+    ctx_union g1 g2 disj_g12 = ctx_union g1 g3 disj_g13.
+
+Proof. Admitted.
+
+Theorem disj_notin_means_disj_with_added :
+  forall g1 g2 g2subv : ty_ctx,
+  forall x : var,
+  forall x_g1free: ~(VarSet.In x g1),
+  forall disj_g12subv : disj_vars g1 g2subv,
+  forall g2subv_def : g2subv = (g2 -- x),
+    disj_vars g1 g2.
+
+Proof. Admitted.
+
 (* Set-Theory Theorems: warning a lot of admits are gonna start being applied for
    things that are obviously true.
  *)
+
+Theorem bound_of_union_is_union_of_bound
+  : forall g1 g2 : ty_ctx,
+    forall disj_g12 : disj_vars g1 g2,
+      bound_variables (ctx_union g1 g2 disj_g12) = VarSet.union (bound_variables g1)
+                                                                (bound_variables g2)
+.
+Proof. Admitted.
+
+Theorem bound_of_restr
+  : forall g : ty_ctx,
+    forall x : var,
+      bound_variables (g -- x) = VarSet.diff (bound_variables g) (VarSet.singleton x).
+Proof. Admitted.
 
 Theorem dvars_distrib :
   forall s1 s2 s3 : ty_ctx,
@@ -100,4 +153,38 @@ Theorem mutuallydisjoint_getsv2 :
   forall disj_g1_g3 : disj_vars g1 g3,
   forall disj_g2_g2 : disj_vars g2 g3,
     disj_vars g1 (bound_variables (ctxu g2 g3)).
+Proof. Admitted.
+
+Theorem in_only_one_of_disjoint :
+  forall g1 g2 : ty_ctx,
+  forall v : var,
+  forall v_in_g2 : VarSet.In v g2,
+  forall disj_g12 : disj_vars g1 g2,
+    ~ (VarSet.In v g1).
+Proof. Admitted.
+
+Theorem not_in_union_means_not_in_either :
+  forall g1 g2 : ty_ctx,
+  forall v : var,
+  forall v_notin_union : ~(VarSet.In v (VarSet.union g1 g2)),
+    ~(VarSet.In v g1).
+Proof. Admitted.
+
+Theorem ctx_union_with_restriction :
+  forall g1 g2 g2subv: ty_ctx,
+  forall v : var,
+  forall v_notin_g1 : ~(VarSet.In v g1),
+  forall g2subv_is_g2_sub_v : (g2subv = (g2 -- v)),
+  forall disj_g12subv : disj_vars g1 g2subv,
+  forall disj_g12 : disj_vars g1 g2,
+    (ctx_union g1 g2subv disj_g12subv) = ((ctx_union g1 g2 disj_g12) -- v).
+Proof. Admitted.
+
+Theorem restriction_from_union_where_notin_one :
+  forall g1 g2 : ty_ctx,
+  forall v : var,
+  forall v_g1free : ~(VarSet.In v g1),
+  forall disj_g12 : disj_vars g1 g2,
+  forall disj_g12subv : disj_vars g1 (g2 -- v),
+    ((ctx_union g1 g2 disj_g12) -- v) = ctx_union g1 (g2 -- v) disj_g12subv.
 Proof. Admitted.
